Move to shallower CTL embedding

AttarchProperties.v
@@ -10,6 +10,7 @@ Require Import AttarchTrans.
 
 Require Import Coq.Program.Equality.
 Require Import Tactics.General.
+Require Import Tactics.Construct.
 
 Definition useram_key_secure : TProp (attarch_global * attarch_state) := 
   ⟨fun st =>
@@ -21,7 +22,7 @@ Theorem useram_key_never_compromised:
   attarch_trans @initial_state_good ⊨ AG useram_key_secure.
 Proof.
   intros n p s' Hin.
-  inhabit in_path__rtc in Hin.
+  construct in_path__rtc in Hin.
   clear p.
   dependent induction Hin.
   - discriminate.
@@ -33,3 +34,16 @@ Proof.
     + invc H1; try apply IHHin.
       invc H0; apply IHHin.
 Qed.
+
+Definition setup_done : TProp (attarch_global * attarch_state) := 
+  ⟨fun st =>
+    snd st = sel4_run (platam_run, vm_run useram_waiting_request)
+  ⟩. 
+
+Theorem useram_key_never_compromised_setup:
+  attarch_trans @initial_state_good ⊨ A[useram_key_secure U setup_done].
+Proof using.
+  (* expand_tEntails. *)
+  intros n p.
+  destruct exists p m.
+  invc p.
