Ctl/Definition.v
@@ -1,83 +1,111 @@
 Require Import Ctl.Paths.
-
 Require Import Coq.Relations.Relation_Definitions.
 
-Inductive TProp state : Type :=
-  | TTop  : TProp state
-  | TBot  : TProp state
-  | TLift : (state -> Prop) -> TProp state
-  | TNot  : TProp state -> TProp state
-  | TConj : TProp state -> TProp state -> TProp state
-  | TDisj : TProp state -> TProp state -> TProp state
-  | TImpl : TProp state -> TProp state -> TProp state
-  | AX    : TProp state -> TProp state
-  | EX    : TProp state -> TProp state
-  | AF    : TProp state -> TProp state
-  | EF    : TProp state -> TProp state
-  | AG    : TProp state -> TProp state
-  | EG    : TProp state -> TProp state
-  | AU    : TProp state -> TProp state -> TProp state
-  | EU    : TProp state -> TProp state -> TProp state.
+(* A very shallow CTL embedding *)
 
-(* Make state argument implicit *)
-Arguments TTop  {state}%type_scope.
-Arguments TBot  {state}%type_scope.
-Arguments TLift {state}%type_scope.
-Arguments TNot  {state}%type_scope.
-Arguments TConj {state}%type_scope.
-Arguments TDisj {state}%type_scope.
-Arguments TImpl {state}%type_scope.
-Arguments AX    {state}%type_scope.
-Arguments EX    {state}%type_scope.
-Arguments AF    {state}%type_scope.
-Arguments EF    {state}%type_scope.
-Arguments AG    {state}%type_scope.
-Arguments EG    {state}%type_scope.
-Arguments AU    {state}%type_scope.
-Arguments EU    {state}%type_scope.
 
-Notation "⊤" := (TTop).
-Notation "⊥" := (TBot).
-Notation "⟨ P ⟩" := (TLift P) (at level 35, format "⟨ P ⟩").
-Notation "P ∧ Q" := (TConj P Q) (at level 45, right associativity).
-Notation "P ∨ Q" := (TDisj P Q) (at level 55, right associativity).
-Notation "P --> Q" := (TImpl P Q) (at level 68,  right associativity).
-Notation "P <--> Q" := ((P --> Q) ∧ (Q --> P)) (at level 65,  right associativity).
-Notation "¬ P" := (TNot P) (at level 40).
-Notation "'A' [ P 'U' Q ]" := (AU P Q) (at level 40, format "'A' [ P  'U'  Q ]").
-Notation "'E' [ P 'U' Q ]" := (EU P Q) (at level 40, format "'E' [ P  'U'  Q ]").
+Definition tprop state := relation state -> state -> Prop.
 
-(* Add "W" operator?
-   "Weak" until, AKA the "unless" operator. Like the until operator, but the
-   second condition does not ever have to come true.
- *)
+Delimit Scope tprop_scope with tprop.
+Open Scope tprop_scope.
 
-Reserved Notation "M @ s ⊨ P" (at level 70, format "M  @ s  ⊨  P").
-Reserved Notation "M @ s ⊭ P" (at level 70, format "M  @ s  ⊭  P").
-(* Replace binary_relation with serial_transition if needed *)
-Fixpoint tEntails {state} (R: relation state) (s: state) (tp: TProp state) : Prop :=
-  match tp with
-  | ⊤ => True
-  | ⊥ => False
-  | ⟨P⟩ => P s
-  | ¬P => R @s ⊭ P
-  | P ∧ Q => R @s ⊨ P /\ R @s ⊨ Q
-  | P ∨ Q => R @s ⊨ P \/ R @s ⊨ Q
-  | P --> Q => R @s ⊨ P -> R @s ⊨ Q
-  | AX P => forall s', R s s' -> R @s' ⊨ P
-  | EX P => exists s', R s s' -> R @s' ⊨ P
-  | AG P => forall n, forall p: path R n s, forall s', in_path s' p -> R @s' ⊨ P
-  | EG P => forall n, exists p: path R n s, forall s', in_path s' p -> R @s' ⊨ P
-  | AF P => exists n, forall p: path R n s, exists s', in_path s' p /\ R @s' ⊨ P
-  | EF P => exists n, exists p: path R n s, exists s', in_path s' p /\ R @s' ⊨ P
-  | A[P U Q] => forall n (p: path R n s),
+Definition tentails {state} (R: relation state) (s: state) (P: tprop state) :=
+  P R s.
+Notation "R @ s ⊨ P" := (tentails R s P) (at level 70, format "R  @ s  ⊨  P") : tprop_scope.
+Notation "R @ s ⊭ P" := (~ tentails R s P) (at level 70, format "R  @ s  ⊭  P") : tprop_scope.
+
+
+(* State props *)
+
+Definition ttop {state}: tprop state :=
+  fun _ _ => True.
+
+Definition tbot {state}: tprop state :=
+  fun _ _ => False.
+Definition tconj {state} (P Q: tprop state): tprop state :=
+  fun R s => R @s ⊨ P /\ R @s ⊨ Q.
+
+Definition tdisj {state} (P Q: tprop state): tprop state := 
+  fun R s => R @s ⊨ P \/ R @s ⊨ Q.
+
+Definition timpl {state} (P Q: tprop state): tprop state :=
+  fun R s => R @s ⊨ P -> R @s ⊨ Q.
+
+Definition tbiimpl {state} (P Q: tprop state): tprop state :=
+  fun R s => R @s ⊨ P <-> R @s ⊨ Q.
+
+Definition tnot {state} (P: tprop state): tprop state :=
+  fun R s => R @s ⊭ P.
+
+(* State prop notations *)
+Notation "⊤" := (ttop) : tprop_scope.
+Notation "⊥" := (tbot) : tprop_scope.
+Notation "P ∧ Q" := (tconj P Q) (at level 45, right associativity) : tprop_scope.
+Notation "P ∨ Q" := (tdisj P Q) (at level 55, right associativity) : tprop_scope.
+Notation "P ⟶ Q" := (timpl P Q) (at level 68,  right associativity) : tprop_scope.
+Notation "P ⟷ Q" := (tbiimpl P Q) (at level 65,  right associativity) : tprop_scope.
+Notation "¬ P" := (tnot P) (at level 40) : tprop_scope.
+
+(* path-quantifying props *)
+
+Definition AX {state} (P: tprop state): tprop state :=
+  fun R s => forall s', R s s' -> R @s' ⊨ P.
+  
+Definition EX {state} (P: tprop state): tprop state :=
+  fun R s => exists s', R s s' /\ R @s' ⊨ P.
+
+Definition AG {state} (P: tprop state): tprop state :=
+  fun R s => forall n (p: path R n s) s', 
+    in_path s' p -> R @s' ⊨ P.
+
+Definition EG {state} (P: tprop state): tprop state :=
+  fun R s => forall n, exists p: path R n s, forall s',
+    in_path s' p -> R @s' ⊨ P.
+
+Definition AF {state} (P: tprop state): tprop state :=
+  fun R s => exists n, forall p: path R n s, exists s',
+    in_path s' p /\ R @ s' ⊨ P.
+
+Definition EF {state} (P: tprop state): tprop state :=
+  fun R s => exists n (p: path R n s) s',
+    in_path s' p /\ R @s' ⊨ P.
+
+Definition AU {state} (P Q: tprop state): tprop state :=
+  fun R s => exists n, forall p: path R n s,
       exists sQ i, in_path_at sQ i p /\ 
         R @sQ ⊨ Q /\
-        forall sP, in_path_before sP i p -> R @sP ⊨ P
-  | E[P U Q] => exists n (p: path R n s),
+        forall sP, in_path_before sP i p -> R @sP ⊨ P.
+
+Definition EU {state} (P Q: tprop state): tprop state :=
+  fun R s => exists n, exists p: path R n s,
       exists sQ i, in_path_at sQ i p /\ 
         R @sQ ⊨ Q /\
-        forall sP, in_path_before sP i p -> R @sP ⊨ P
-  end
-  where "M @ s ⊨ P" := (tEntails M s P)
-    and "M @ s ⊭ P" := (~ M @s ⊨ P).
+        forall sP, in_path_before sP i p -> R @sP ⊨ P.
+
+Definition AW {state} (P Q: tprop state): tprop state :=
+  fun R s => forall n (p: path R n s) y i,
+      in_path_at y i p ->
+      (forall x,
+        in_path_before x i p ->
+        R @x ⊨ P ∧ ¬Q) ->
+      R @y ⊨ P ∨ Q.
+
+(* Path-quantifying prop notations *)
+Notation "A[ P 'U' Q ]" := (AU P Q) (at level 40, format "A[ P  'U'  Q ]") : tprop_scope.
+Notation "E[ P 'U' Q ]" := (EU P Q) (at level 40, format "E[ P  'U'  Q ]") : tprop_scope.
+Notation "A[ P 'W' Q ]" := (AW P Q) (at level 40, format "A[ P  'W'  Q ]") : tprop_scope.
+
+Global Opaque tentails.
+Global Opaque ttop.
+Global Opaque tbot.
+Global Opaque tconj.
+Global Opaque tdisj.
+Global Opaque timpl.
+Global Opaque tbiimpl.
+Global Opaque AX.
+Global Opaque EX.
+Global Opaque AF.
+Global Opaque EF.
+Global Opaque AU.
+Global Opaque EU.
+Global Opaque AW.
