BinaryRelations.v
@@ -6,6 +6,7 @@ Require Import Setoid.
 Require Import Psatz.
 Require Import Coq.Program.Equality.
 Require Import Tactics.General.
+Require Import Tactics.Construct.
 
 Definition is_serial {A} (R: relation A) := forall a, exists b, R a b.
 Definition serial A := {R: relation A | is_serial R}.
@@ -317,22 +318,22 @@ Definition in_rtcT_idx_before {state} {R: relation state} {n s s'}
 
 Theorem in_rtcT_idx__prefix {state}: 
   forall (R: relation state) x y z n (Rxz: R^# n x z),
-    in_rtcT_idx y Rxz ->
-    inhabited {m & m <= n & R^# m x y}.
+    in_rtcT_idx y Rxz ~>
+    {m & m <= n & R^# m x y}.
 Proof using.
   introv H.
   dependent induction H.
-  - constructor.
+  - construct.
     exists 0.
     + reflexivity.
     + constructor.
-  - constructor.
+  - construct.
     exists (S n).
     + reflexivity.
     + econstructor; eassumption.
-  - invc IHin_rtcT_idx.
-    destruct exists X m.
-    constructor.
+  - uninhabit IHin_rtcT_idx.
+    destruct exists IHin_rtcT_idx m.
+    construct.
     exists m.
     + constructor. assumption.
     + assumption.
@@ -340,13 +341,13 @@ Qed.
  
 Theorem in_rtcT_idx__prefix' {state}: 
   forall (R: relation state) x y z n (Rxz: R^# n x z),
-    in_rtcT_idx y Rxz ->
-    inhabited (R^* x y).
+    in_rtcT_idx y Rxz ~>
+    R^* x y.
 Proof using.
   introv H.
   dependent induction H.
-  - repeat constructor. 
-  - constructor.
+  - construct. constructor. 
+  - construct.
     econstructor.
     + eassumption.
     + eapply rtcT_idx_to_rtcT.
