Classical.v
@@ -1,0 +1,12 @@
+Require Import Coq.Logic.Classical.
+
+Theorem destruct_impl : forall p q,
+  ~p \/ p /\ q <-> (p -> q).
+Proof using.
+  intros p q.
+  split; intro H.
+  - destruct H.
+    + intro Hp. contradiction.
+    + intro H1. apply H.
+  - destruct (classic p); auto.
+Qed.
