Ctl/Basic.v
@@ -1,0 +1,122 @@
+Require Import Ctl.Paths.
+Require Import Ctl.Definition.
+Open Scope tprop_scope.
+
+Require Import Coq.Relations.Relation_Definitions.
+
+
+Theorem tentails_ttop {state}: forall (R: relation state) s,
+  R @s ⊨ ⊤.
+Proof using. intros; exact I. Qed.
+
+Theorem ntentails_tbot {state}: forall (R: relation state) s,
+  R @s ⊭ ⊥.
+Proof using. auto. Qed.
+
+Theorem tentails_tconj {state}: forall (R: relation state) s P Q,
+  R @s ⊨ P ->
+  R @s ⊨ Q ->
+  R @s ⊨ P ∧ Q.
+Proof using. 
+  intros.
+  split; assumption.
+Qed.
+
+Theorem rew_tconj {state}: forall (R: relation state) s P Q,
+  R @s ⊨ P ∧ Q =
+  (R @s ⊨ P /\ R @s ⊨ Q).
+Proof using. reflexivity. Qed.
+
+Theorem tentails_tdisj_l {state}: forall (R: relation state) s P Q,
+  R @s ⊨ P ->
+  R @s ⊨ P ∨ Q.
+Proof using.
+  intros.
+  left.
+  assumption.
+Qed.
+
+Theorem tentails_tdisj_r {state}: forall (R: relation state) s P Q,
+  R @s ⊨ Q ->
+  R @s ⊨ P ∨ Q.
+Proof using.
+  intros.
+  right.
+  assumption. 
+Qed.
+
+Theorem rew_tdisj {state}: forall (R: relation state) s P Q,
+  R @s ⊨ P ∨ Q = 
+  (R @s ⊨ P \/ R @s ⊨ Q).
+Proof using. reflexivity. Qed.
+
+Theorem rew_timpl {state}: forall (R: relation state) s P Q,
+  R @s ⊨ P ⟶ Q =
+  (R @s ⊨ P -> R @s ⊨ Q).
+Proof using. reflexivity. Qed.
+
+Theorem rew_tbiimpl {state}: forall (R: relation state) s P Q,
+  R @s ⊨ P ⟷ Q =
+  (R @s ⊨ P <-> R @s ⊨ Q).
+Proof using. reflexivity. Qed.
+
+Theorem rew_tnot {state}: forall (R: relation state) s P,
+  R @s ⊨ ¬ P =
+  (R @s ⊭ P).
+Proof using. reflexivity. Qed.
+
+Theorem rew_AX {state}: forall (R: relation state) s P,
+  R @s ⊨ AX P =
+  forall s', R s s' -> R @s' ⊨ P.
+Proof using. reflexivity. Qed. 
+
+Theorem rew_EX {state}: forall (R: relation state) s P,
+  R @s ⊨ EX P =
+  exists s', R s s' /\ R @s' ⊨ P.
+Proof using. reflexivity. Qed. 
+
+Theorem rew_AG {state}: forall (R: relation state) s P,
+  R @s ⊨ AG P =
+  forall n (p: path R n s) s', in_path s' p -> R @s' ⊨ P.
+Proof using. reflexivity. Qed.
+
+Theorem rew_EG {state}: forall (R: relation state) s P,
+  R @s ⊨ EG P = 
+  forall n, exists p: path R n s, forall s', in_path s' p -> R @s' ⊨ P.
+Proof using. reflexivity. Qed.
+
+Theorem rew_AF {state}: forall (R: relation state) s P,
+  R @s ⊨ AF P = 
+  exists n, forall p: path R n s, exists s', in_path s' p /\ R @s' ⊨ P.
+Proof using. reflexivity. Qed.
+
+Theorem rew_EF {state}: forall (R: relation state) s P,
+  R @s ⊨ EF P =
+  exists n (p: path R n s) s', in_path s' p /\ R @s' ⊨ P.
+Proof using. reflexivity. Qed.
+
+Theorem rew_AU {state}: forall (R: relation state) s P Q,
+  R @s ⊨ A[P U Q] =  
+  exists n, forall p: path R n s, exists sQ i,
+    in_path_at sQ i p /\ 
+    R @sQ ⊨ Q /\
+    forall sP, in_path_before sP i p -> R @sP ⊨ P.
+Proof using. reflexivity. Qed.
+
+Theorem rew_EU {state}: forall (R: relation state) s P Q,
+  R @s ⊨ E[P U Q] =
+  exists n (p: path R n s) sQ i,
+    in_path_at sQ i p /\ 
+    R @sQ ⊨ Q /\
+    forall sP, in_path_before sP i p -> R @sP ⊨ P.
+Proof using. reflexivity. Qed.
+
+Theorem rew_AW {state}: forall (R: relation state) s P Q,
+  R @s ⊨ A[P W Q] =
+  forall n (p: path R n s) y i,
+    in_path_at y i p ->
+    (forall x,
+      in_path_before x i p ->
+      R @x ⊨ P ∧ ¬Q) ->
+    R @y ⊨ P ∨ Q.
+Proof using. reflexivity. Qed.
